bfn.v
@@ -14,15 +14,67 @@ Module BFN.
   | bfn_in : nat -> BFN -> BFN    (* , *)
   | bfn_loop : BFN -> BFN -> BFN.  (* [...] *)
 
+  (* BFN Semantics *)
+  Definition BFNState := @BFTape.ExecState BFN.
+  Definition state := @BFTape.state BFN.
 
-  Fixpoint repeat_com (fn : BF -> BF) (n : nat) (bf: BF) : BF :=
+  Function bfn_step (s: BFNState): option BFNState :=
+    match s with
+    | BFTape.state bfn resets ptr tape input output =>
+      match bfn with
+      | bfn_end =>
+        match resets with
+        | [] => None
+        | bfn' :: resets' =>
+          Some (state bfn' resets' ptr tape input output)
+        end
+      | bfn_right n bfn' =>
+        Some (state bfn' resets (ptr + n) tape input output)
+      | bfn_left n bfn' =>
+        Some (state bfn' resets (ptr - n) tape input output)
+      | bfn_inc n bfn' =>
+        Some (state bfn' resets ptr
+                    (BFTape.put tape ptr ((BFTape.get tape ptr) + n))
+                    input output)
+      | bfn_dec n bfn' =>
+        Some (state bfn' resets ptr
+                    (BFTape.put tape ptr ((BFTape.get tape ptr) - n))
+                    input output)
+      | bfn_out (S n) bfn' =>
+        Some (state (bfn_out n bfn') resets ptr tape input
+                    (output ++ [BFTape.get tape ptr]))
+      | bfn_in (S n) bfn' =>
+        match input with
+        | [] =>
+          Some (state (bfn_in n bfn') resets ptr (BFTape.put tape ptr 0)
+                      input output)
+        | x :: input' =>
+          Some (state (bfn_in n bfn') resets ptr (BFTape.put tape ptr x)
+                      input' output)
+        end
+      | bfn_out 0 bfn'
+      | bfn_in 0 bfn' => Some (state bfn' resets ptr tape input output)
+      | bfn_loop inner_bfn bfn' =>
+        if (BFTape.get tape ptr) =? 0 then
+          Some (state bfn' resets ptr tape input output)
+        else
+          Some (state inner_bfn (bfn :: resets) ptr tape input output)
+      end
+    end.
+
+  (* Key function for translation correctness *)
+  Definition interpret_bfn (prog: BFN) (input: list nat) (fuel: nat):
+    option (list nat) := BFTape.interpret bfn_step prog input fuel.
+
+  (* Translation BFN -> BF *)
+  Function repeat_com (fn : BF -> BF) (n : nat) (bf: BF) : BF :=
     match n with
     | 0 => bf_end  (* should probably not be used *)
     | 1 => fn bf
     | S m => fn (repeat_com fn m bf)
     end.
 
-  Fixpoint bf_of_bfn (bfn: BFN): BF :=
+  Function bf_of_bfn (bfn: BFN): BF :=
     match bfn with
     | bfn_end => bf_end
     | bfn_right n bfn' => repeat_com bf_right n (bf_of_bfn bfn')
@@ -34,9 +86,22 @@ Module BFN.
     | bfn_loop bfn1 bfn2 => bf_loop (bf_of_bfn bfn1) (bf_of_bfn bfn2)
     end.
 
-  Example parse_left_bfn:
+  Example translate_left_bfn:
     parse_bf "<<<<+++++++" =
     Some (bf_of_bfn (bfn_left 4 (bfn_inc 7 bfn_end))).
   auto. Qed.
+
+  (* TODO: Prove bf_of_bfn_correct *)
+  Lemma bf_of_bfn_correct:
+    forall (bfn: BFN) (input output: list nat),
+      (exists fuel, interpret_bfn bfn input fuel = Some output) ->
+      (exists fuel, interpret_bf (bf_of_bfn bfn) input fuel = Some output).
+  Proof.
+    intros.
+    destruct H.
+    functional induction (bf_of_bfn bfn).
+    - destruct x; compute in H; try discriminate.
+      exists 1; auto.
+  Admitted.
 
 End BFN.
