bftape.v
@@ -25,7 +25,9 @@ Module BFTape.
   Definition dec (tape: Tape) (ptr: nat): Tape :=
     put tape ptr (pred (get tape ptr)).
 
-  (* Tape language execution state *)
+  (* Tape language execution state.
+     `ast' is the current state of the program, while `resets' is the
+     stack of programs to reset to at the end of a loop *)
   Inductive ExecState {A: Type} : Type :=
     state (ast: A)
           (resets: list A)
@@ -34,10 +36,26 @@ Module BFTape.
           (input: list nat)
           (output: list nat).
 
-  Function exec_init {A: Type} (bf: A) (input: list nat): ExecState :=
-    state bf [] 0 BFTape.empty input [].
+  Function exec_init {A: Type} (prog: A) (input: list nat): ExecState :=
+    state prog [] 0 BFTape.empty input [].
 
   Function exec_output {A: Type } (state: @ExecState A): list nat :=
     match state with state _ _ _ _ _ output => output end.
+
+  (* TODO: Use N as fuel with {measure N.to_nat fuel} *)
+  Function run {A: Type} (step: @ExecState A -> option (@ExecState A))
+           (state: @ExecState A) (fuel: nat): option (list nat) :=
+    match fuel with
+    | 0 => None
+    | S f =>
+      match step state with
+      | None => Some (exec_output state)
+      | Some state' => run step state' f
+      end
+    end.
+
+  Definition interpret {A: Type} (step: @ExecState A -> option (@ExecState A))
+           (prog: A) (input: list nat) (fuel: nat): option (list nat) :=
+    run step (exec_init prog input) fuel.
 
 End BFTape.
